src/impl/TLS13.Impl.Handle.ChangeCipherSpec.fst
@@ -30,50 +30,104 @@ fn handle_change_cipher_spec
            pts_to app_out 'old_app_out **
            pure (B.length 'raw_bytes == SZ.v raw_len /\
                  B.length 'old_network_out == SZ.v network_out_len /\
-           B.length 'old_app_out == SZ.v app_out_len /\
-           L.tls_message_is_change_cipher_spec l)
+                 B.length 'old_app_out == SZ.v app_out_len /\
+                 L.tls_message_is_change_cipher_spec l /\
+                 CT.received_tls_raw_delta_legal
+                   'st0
+                   M.TlsChangeCipherSpec
+                   (Ghost.reveal 'raw_bytes))
   returns resp: CT.client_response
-  ensures C.connection_exactly c (C.local_fail_state 'st0 C.tls_unexpected_message_error) **
+  ensures exists* st1.
+          C.connection_exactly c st1 **
           pts_to raw 'raw_bytes **
           pts_to network_out 'old_network_out **
           pts_to app_out 'old_app_out **
           pure (B.length 'old_network_out == SZ.v network_out_len /\
                 B.length 'old_app_out == SZ.v app_out_len /\
-                CT.unexpected_message_response
+                CT.legal_handled_tls_response
                   'st0
-                  (C.local_fail_state 'st0 C.tls_unexpected_message_error)
+                  st1
                   resp
+                  M.TlsChangeCipherSpec
+                  (Ghost.reveal 'raw_bytes)
                   'old_network_out
                   'old_app_out /\
                 CT.some_legal_response
                   'st0
-                  (C.local_fail_state 'st0 C.tls_unexpected_message_error)
+                  st1
                   resp
                   'old_network_out
                   'old_app_out)
 {
-  with m. assert (pure True);
-  L.free_tls_message l;
-  C.mark_unexpected_message c;
-  let resp = {
-    CT.network_out_len = 0sz;
-    CT.app_out_len = 0sz;
-    CT.status = CT.IllegalTransition;
-  };
-  Seq.lemma_len_slice 'old_network_out 0 0;
-  Seq.lemma_eq_intro B.empty (Seq.slice 'old_network_out 0 0);
-  assert (pure (Seq.equal B.empty (CT.response_network_out resp 'old_network_out)));
-  assert (pure (CT.unexpected_message_response
-    'st0
-    (C.local_fail_state 'st0 C.tls_unexpected_message_error)
-    resp
-    'old_network_out
-    'old_app_out));
-  assert (pure (CT.some_legal_response
-    'st0
-    (C.local_fail_state 'st0 C.tls_unexpected_message_error)
-    resp
-    'old_network_out
-    'old_app_out));
-  resp
+  let handshaking = C.is_handshaking c;
+  if handshaking {
+   with m. assert (pure True);
+   L.free_tls_message l;
+   C.mark_received_change_cipher_spec c raw;
+   let resp = {
+     CT.network_out_len = 0sz;
+     CT.app_out_len = 0sz;
+     CT.status = CT.StepOk;
+   };
+   Seq.lemma_len_slice 'old_network_out 0 0;
+   Seq.lemma_eq_intro B.empty (Seq.slice 'old_network_out 0 0);
+   assert (pure (Seq.equal B.empty (CT.response_network_out resp 'old_network_out)));
+   C.lemma_received_change_cipher_spec_state_evolves 'st0 (Ghost.reveal 'raw_bytes);
+   assert (pure (CT.legal_received_tls_response
+     'st0
+     (C.received_change_cipher_spec_state 'st0 (Ghost.reveal 'raw_bytes))
+     resp
+     M.TlsChangeCipherSpec
+     (Ghost.reveal 'raw_bytes)
+     'old_network_out
+     'old_app_out));
+   assert (pure (CT.legal_handled_tls_response
+     'st0
+     (C.received_change_cipher_spec_state 'st0 (Ghost.reveal 'raw_bytes))
+     resp
+     M.TlsChangeCipherSpec
+     (Ghost.reveal 'raw_bytes)
+     'old_network_out
+     'old_app_out));
+   assert (pure (CT.some_legal_response
+     'st0
+     (C.received_change_cipher_spec_state 'st0 (Ghost.reveal 'raw_bytes))
+     resp
+     'old_network_out
+     'old_app_out));
+   resp
+  } else {
+   with m. assert (pure True);
+   L.free_tls_message l;
+   C.mark_unexpected_message c;
+   let resp = {
+     CT.network_out_len = 0sz;
+     CT.app_out_len = 0sz;
+     CT.status = CT.IllegalTransition;
+   };
+   Seq.lemma_len_slice 'old_network_out 0 0;
+   Seq.lemma_eq_intro B.empty (Seq.slice 'old_network_out 0 0);
+   assert (pure (Seq.equal B.empty (CT.response_network_out resp 'old_network_out)));
+   assert (pure (CT.unexpected_message_response
+     'st0
+     (C.local_fail_state 'st0 C.tls_unexpected_message_error)
+     resp
+     'old_network_out
+     'old_app_out));
+   assert (pure (CT.legal_handled_tls_response
+     'st0
+     (C.local_fail_state 'st0 C.tls_unexpected_message_error)
+     resp
+     M.TlsChangeCipherSpec
+     (Ghost.reveal 'raw_bytes)
+     'old_network_out
+     'old_app_out));
+   assert (pure (CT.some_legal_response
+     'st0
+     (C.local_fail_state 'st0 C.tls_unexpected_message_error)
+     resp
+     'old_network_out
+     'old_app_out));
+   resp
+  }
 }
