src/impl/TLS13.Impl.Handle.Dispatch.fst
@@ -45,7 +45,11 @@ fn dispatch_network_event
                       WS.parse_tls_message ct 'fragment_bytes == Some m)) **
               pure (exists ct msg.
                 L.content_type_matches content_type ct /\
-                WS.parse_tls_message ct 'fragment_bytes == Some msg)
+                WS.parse_tls_message ct 'fragment_bytes == Some msg) **
+              pure (CT.parsed_message_wire_success
+                content_type
+                (Ghost.reveal 'fragment_bytes)
+                l)
             | None ->
               pure (forall (ct:T.content_type).
                 L.content_type_matches content_type ct ==>
@@ -53,7 +57,12 @@ fn dispatch_network_event
            pure (B.length 'raw_bytes == SZ.v raw_len /\
                  B.length 'fragment_bytes == SZ.v fragment_len /\
                  B.length 'old_network_out == SZ.v network_out_len /\
-                 B.length 'old_app_out == SZ.v app_out_len)
+                 B.length 'old_app_out == SZ.v app_out_len /\
+                 CT.network_input_wf
+                   'st0
+                   content_type
+                   (Ghost.reveal 'fragment_bytes)
+                   (Ghost.reveal 'raw_bytes))
   returns resp: CT.client_response
   ensures exists* st1 network_out_bytes app_out_bytes.
           C.connection_exactly c st1 **
@@ -165,6 +174,18 @@ fn dispatch_network_event
           resp
         }
         L.LTlsChangeCipherSpec -> {
+          assert (pure (CT.parsed_message_wire_success
+            content_type
+            (Ghost.reveal 'fragment_bytes)
+            L.LTlsChangeCipherSpec));
+          assert (pure (CT.wire_parse_success
+            content_type
+            (Ghost.reveal 'fragment_bytes)
+            M.TlsChangeCipherSpec));
+          assert (pure (CT.received_tls_raw_delta_legal
+            'st0
+            M.TlsChangeCipherSpec
+            (Ghost.reveal 'raw_bytes)));
           let resp =
             HChangeCipherSpec.handle_change_cipher_spec
               c
@@ -175,15 +196,6 @@ fn dispatch_network_event
               network_out_len
               app_out
               app_out_len;
-          CT.lemma_legal_network_response_unexpected_from_parse_success
-            'st0
-            (C.local_fail_state 'st0 C.tls_unexpected_message_error)
-            resp
-            content_type
-            (Ghost.reveal 'fragment_bytes)
-            (Ghost.reveal 'raw_bytes)
-            'old_network_out
-            'old_app_out;
           resp
         }
       }
